--- 
title: "A comment about the integral representation of the Riemann xi-function"
author: "George Pólya"
date: "1926"
original: 'Pólya, G. "Bemerkung Über die Integraldarstellung der Riemannschen $\xi$-Funktion". _Acta Math._ **48** (1926), 305--317. DOI: [10.1007/BF02565336](https://doi.org/10.1007/BF02565336).'
github-repo: "thosgood/translations"
favicon: "favicon.ico"
---

```{js, echo = FALSE}
$(document).ready(function(e) {gitbook.sidebar.toggle(false, false)});
```

```{r, child = '_translator-note.Rmd'}
```

\providecommand{\scr}[1]{{\mathscr{#1}}}
\renewcommand{\cal}[1]{{\mathcal{#1}}}
\renewcommand{\frak}[1]{{\mathfrak{#1}}}
\renewcommand{\geq}{\geqslant}
\renewcommand{\leq}{\leqslant}

<!-- Shortcuts -->

\newcommand{\dd}{\operatorname{d}\!}
\newcommand{\GG}{\frak{G}}
\newcommand{\UU}{\scr{U}}
\newcommand{\TT}{\scr{T}}
\renewcommand{\SS}{\scr{S}}
\newcommand{\error}{\cal{O}}

<!-- Content -->

*[Translator.] The numbering of the footnotes in the original has not been replicated in this translation, since this would have resulted in multiple footnotes with the same number on one page. We also thank [Juan Arias de Reyna](https://personal.us.es/arias/) for their Spanish translation of this paper, which helped greatly.*

The Riemann $\xi$-function, defined by the formula
\oldpage{305}
$$
  \xi(iz)
  =
  \frac12 \left(
    z^2 - \frac14
  \right) \pi^{-\frac{z}{2}-\frac14} \Gamma \left(
    \frac{z}{2} + \frac14
  \right) \zeta \left(
    \frac12 + z
  \right),
\tag{1}
$$
was represented by Riemann himself by an infinite trigonometric integral, namely^[B. Riemann, Werke (1876), S. 138.]
$$
  \xi(z) = 2\int_0^\infty \Phi(u)\cos(zu)\dd u
\tag{2}
$$
$$
  \Phi(u) = 2\pi e^{\frac{5u}{2}} \sum_{n=1}^\infty (2\pi e^{2u}n^2 - 3) n^2 e^{-n^2\pi e^{2u}}.
\tag{3}
$$
It is evident that
$$
  \Phi(u) \sim 4\pi^2 e^{\frac{9u}{2}-\pi e^{2u}}
  \quad\text{as }u\to+\infty.
\tag{4}
$$
Furthermore (see [§4](#section-4)), $\Phi(u)$ is an even function.
Therefore
$$
  \Phi(u) \sim 4\pi^2 \left(
    e^{\frac{9u}{2}} + e^{-\frac{9u}{2}}
  \right) e^{-\pi(e^{2u}+e^{-2u})}
  \quad\text{as }u\to\pm\infty.
\tag{5}
$$

\oldpage{306}
With regards to the Riemann hypothesis, one could ask the following question^[This was casually mentioned by Prof. Landau in a conversation in 1913.]: does the function given by replacing $\Phi(u)$ in the right-hand side of Equation (2) with the right-hand side of Equation (4) have only real zeros?

The answer is no (see [§4](#section-4)): the resulting function has infinitely many imaginary zeros.
If, however, the right-hand side of Equation (5) is used, instead of the right-hand side of Equation (4), then we obtain the function
$$
  \xi^*(z) = 8\pi^2 \int_0^\infty \left(
    e^{\frac{9u}{2}} + e^{-\frac{9u}{2}}
  \right) e^{-\pi(e^{2u}+e^{-2u})} \cos(zu) \dd u,
\tag{6}
$$
which one could call the "modified $\xi$-function", and $\xi^*(z)$ in fact *has only real zeros*.
Incidentally,
$$
  \xi(z) \sim \xi^*(z)
$$
if $z$ tends towards $\infty$ in some closed ray based at the point $0$ and not containing the real axis.
If we denote by $N(r)$ the number of zeros of $\xi(z)$ in the circular region $|z|\leq r$, and by $N^*(r)$ the number of zeros of $\xi^*(z)$ in the same region, then
$$
  N(r) \sim N^*(r)
$$
and even
$$
  N(r) - N^*(r) = O(\log r).
$$

In what follows, I provide a proof of the fact that all the zeros of $\xi^*(z)$ are real.
The proof focuses on another entire function, namely the function
$$
  \GG(z) = \GG(z;a) = \int_{-\infty}^{+\infty} e^{-a(e^u+e^{-u})+zu} \dd u,
\tag{7}
$$
which has some nice, simple properties.
The parameter $a$ is always a positive value.
We can express $\xi^*(z)$ in terms of $\GG(z)$.
\oldpage{307}
Indeed,
$$
  \xi^*(z) = 2\pi^2 \left\{
    \GG\left(
      \frac{iz}{2} - \frac94; \pi
    \right) +
    \GG\left(
      \frac{iz}{2} + \frac94; \pi
    \right)
  \right\}
\tag{8}
$$
as one can easily derive from Equations (6) and (7).
I will show that $\GG(iz)$ *has only real zeros*.
From this, the same property then easily follows for $\xi^*(z)$.


# 1 {.unnumbered #section-1}

The most important property of the entire function $\GG(z)$ is that is satisfies a simple difference equation;
namely
$$
  z\GG(z) = a(\GG(z+1) - \GG(z-1))
\tag{9}
$$
as can easily be proven by partial integration.
Note also that $\GG(z)$ is even:
$$
  \GG(-z) = \GG(z).
\tag{10}
$$
Furthermore, if $z$ is not an integer, then
$$
  \begin{aligned}
    \GG(z)
    &= a^{-z}\Gamma(z) \left(
      1 + \sum_{n=1}^\infty \frac{a^{2n}}{n!(1-z)(2-z)\ldots(n-z)}
    \right)
  \\&+ a^z\Gamma(-z) \left(
      1 + \sum_{n=1}^\infty \frac{a^{2n}}{n!(1+z)(2+z)\ldots(n+z)}
    \right).
  \end{aligned}
\tag{11}
$$

The proof of Equation (11) goes as follows: write
$$
  \Gamma(z)
  = \int_0^a e^{-v} v^{z-1} \dd v + \int_a^\infty e^{-v} v^{z-1} \dd v
  = P(z) + Q(z),
\tag{12}
$$
$$
  P(z) = P(z;a) = \sum_{n=0}^\infty \frac{(-1)^n a^{z+n}}{n!(z+n)},
\tag{13}
$$
$$
  Q(z) = Q(z;a) = a^z \int_0^\infty e^{-ae^u+uz} \dd u.
\tag{14}
$$

Now,
$$
  \begin{aligned}
    \GG(z)
    &= \int_0^\infty e^{-a(e^u+e^{-u})} (e^{uz}+e^{-uz}) \dd u
  \\&= \int_0^\infty \sum_{n=0}^\infty e^{-ae^u} \frac{(-a)^n}{n!} (e^{(-n+z)u}+e^{(-n-z)u}) \dd u.
  \end{aligned}
$$
From this it follows, by Equation (14), after exchanging the order of summation and integration (which can easily be justified by absolute convergence), that
\oldpage{308}
$$
  \GG(z)
  = a^{-z}\sum_{n=0}^\infty \frac{(-1)^n a^{2n}}{n!} Q(-n+z)
  + a^z\sum_{n=0}^\infty \frac{(-1)^n a^{2n}}{n!} Q(-n-z).
\tag{15}
$$
On the other hand, evidently
$$
  \begin{aligned}
    0
    &= \sum_{k=0}^\infty \sum_{l=0}^\infty \frac{(-1)^{k+l}a^{k+l}}{k!l!} \left(
      \frac{1}{-k+z+l} + \frac{1}{k-z-l}
    \right)
  \\&= a^{-z} \sum_{k=0}^\infty \frac{(-1)^ka^{2k}}{k!} \sum_{l=0}^\infty \frac{(-1)^la^{-k+z+l}}{l!(-k+z+l)}
  \\&+ a^z \sum_{l=0}^\infty \frac{(-1)^la^{2l}}{l!} \sum_{k=0}^\infty \frac{(-1)^ka^{-l-z+k}}{k!(-l-z+k)}
  \end{aligned}
$$
and so, by Equation (13),
$$
  \GG(z)
  = a^{-z} \sum_{k=0}^\infty \frac{(-1)^ka^{2k}}{k!} P(-k+z)
  + a^z \sum_{l=0}^\infty \frac{(-1)^la^{2l}}{l!} P(-l-z).
\tag{16}
$$
It follows from Equations (12), (15), and (16) that
$$
  \GG(z)
  = a^{-z} \sum_{n=0}^\infty \frac{(-1)^na^{2n}}{n!} \Gamma(-n+z)
  + a^z \sum_{n=0}^\infty \frac{(-1)^na^{2n}}{n!} \Gamma(-n-z),
$$
which is equivalent to Equation (11).

I will also state here, without proof, the two following representations, which will not be used in what follows:
$$
  \begin{aligned}
    \GG(z)
    &= \frac{1}{2\pi i} \int_{a-i\infty}^{a+i\infty} \Gamma\left(
      s - \frac{z}{2}
    \right) \Gamma \left(
      s + \frac{z}{2}
    \right) a^{-2s} \dd s,
  \\\GG(z)
    &= \frac{\pi}{\sin(\pi z)} e^{\frac{i\pi z}{2}} J_{-z}(2ia) - \frac{\pi}{\sin(\pi z)} e^{-\frac{i\pi z}{2}} J_z(2ia).
  \end{aligned}
$$
In the first one, $2a>|\Re z|$; in the second, both terms on the right-hand side satisfy the same difference equation, which is also satisfied by $\GG(z)$, by Equation (9).


